Veir/Dialects/Arith/OpInfo.lean
@@ -94,7 +94,7 @@ def Arith.toAttrDict
         (Attribute.arithIntegerOverflowFlagsAttr props.attr)
     dict
   | .cmpi =>
-    let value := IntegerAttr.mk (Int.ofNat props.predicate.toNat) (IntegerType.mk 64)
+    let value := IntegerAttr.ofInt (Int.ofNat props.predicate.toNat) (IntegerType.mk 64)
     (Std.HashMap.emptyWithCapacity 1).insert
       "predicate".toUTF8 (Attribute.integerAttr value)
   | .divsi | .divui | .shrsi | .shrui => Id.run do
@@ -162,7 +162,7 @@ def Arith.materializeConstant {OpInfo : Type} [HasOpInfo OpInfo] [HasDialect OpI
   match value, type.val with
   | .int bw (.val value), .integerType intType =>
     if bw = intType.bitwidth then
-      some (.of Arith.constant (ArithConstantProperties.mk (IntegerAttr.mk value.toInt intType)))
+      some (.of Arith.constant (ArithConstantProperties.mk (IntegerAttr.ofInt value.toInt intType)))
     else none
   | .int bw .poison, .integerType intType =>
     if bw = intType.bitwidth then some (.of Llvm.mlir__poison ()) else none
