Test/Passes/InstructionSelection/RISCV64/sext.mlir
@@ -20,12 +20,12 @@
         // CHECK-NEXT:      %[[M:.*]] = "riscv.sextw"(%[[L]]) : (!riscv.reg) -> !riscv.reg
         // CHECK-NEXT:      %[[N:.*]] = "builtin.unrealized_conversion_cast"(%[[M]]) : (!riscv.reg) -> i64
         // CHECK-NEXT:      %[[O:.*]] = "builtin.unrealized_conversion_cast"([[A]]) : (i1) -> !riscv.reg
-        // CHECK-NEXT:      %[[P:.*]] = "riscv.slli"(%[[O]]) <{"value" = 63 : i6}> : (!riscv.reg) -> !riscv.reg
-        // CHECK-NEXT:      %[[Q:.*]] = "riscv.srai"(%[[P]]) <{"value" = 63 : i6}> : (!riscv.reg) -> !riscv.reg
+        // CHECK-NEXT:      %[[P:.*]] = "riscv.slli"(%[[O]]) <{"value" = -1 : i6}> : (!riscv.reg) -> !riscv.reg
+        // CHECK-NEXT:      %[[Q:.*]] = "riscv.srai"(%[[P]]) <{"value" = -1 : i6}> : (!riscv.reg) -> !riscv.reg
         // CHECK-NEXT:      %[[R:.*]] = "builtin.unrealized_conversion_cast"(%[[Q]]) : (!riscv.reg) -> i64
         // CHECK-NEXT:      %[[S:.*]] = "builtin.unrealized_conversion_cast"([[A]]) : (i1) -> !riscv.reg
-        // CHECK-NEXT:      %[[T:.*]] = "riscv.slli"(%[[S]]) <{"value" = 63 : i6}> : (!riscv.reg) -> !riscv.reg
-        // CHECK-NEXT:      %[[U:.*]] = "riscv.srai"(%[[T]]) <{"value" = 63 : i6}> : (!riscv.reg) -> !riscv.reg
+        // CHECK-NEXT:      %[[T:.*]] = "riscv.slli"(%[[S]]) <{"value" = -1 : i6}> : (!riscv.reg) -> !riscv.reg
+        // CHECK-NEXT:      %[[U:.*]] = "riscv.srai"(%[[T]]) <{"value" = -1 : i6}> : (!riscv.reg) -> !riscv.reg
         // CHECK-NEXT:      %[[V:.*]] = "builtin.unrealized_conversion_cast"(%[[U]]) : (!riscv.reg) -> i32
         // CHECK-NEXT:      %[[W:.*]] = "builtin.unrealized_conversion_cast"([[E]]) : (i8) -> !riscv.reg
         // CHECK-NEXT:      %[[X:.*]] = "riscv.sextb"(%[[W]]) : (!riscv.reg) -> !riscv.reg
